Impl/QueryModel.i.dfy
@@ -1,5 +1,5 @@
 include "StateModel.i.dfy"
-include "CacheModel.i.dfy"
+include "BookkeepingModel.i.dfy"
 include "../lib/Base/Option.s.dfy"
 include "../lib/Base/Sets.i.dfy"
 include "../PivotBetree/PivotBetreeSpec.i.dfy"
@@ -9,7 +9,7 @@ include "../PivotBetree/PivotBetreeSpec.i.dfy"
 module QueryModel { 
   import opened StateModel
   import opened IOModel
-  import opened CacheModel
+  import opened BookkeepingModel
 
   import opened Options
   import opened Maps
